submission from Fang

HOTG/Arithmetics/Less_Than.thy
@@ -16,14 +16,33 @@ bundle no_hotg_lt_syntax begin no_notation lt (infix "<" 60) end
 unbundle hotg_lt_syntax
 unbundle no_HOL_order_syntax
 
+definition le (infix "\<le>" 50) 
+  where "X \<le> Y \<equiv> X < Y \<or> X = Y"
+
 lemma lt_iff_mem_trans_closure: "X < Y \<longleftrightarrow> X \<in> mem_trans_closure Y"
   unfolding lt_def by simp
+
+lemma le_iff_mem_trans_closure_or_eq: "X \<le> Y \<longleftrightarrow> X \<in> mem_trans_closure Y \<or> X = Y"
+  by (simp add: le_def lt_iff_mem_trans_closure)
 
 lemma lt_if_lt_if_mem [trans]:
   assumes "y \<in> Y"
   and "Y < X"
   shows "y < X"
   using assms mem_trans_closed_mem_trans_closure unfolding lt_iff_mem_trans_closure by auto
+
+lemma lt_if_lt_if_mem_strong [trans]:
+  assumes "y < Y"
+  and "Y < X"
+shows "y < X"
+  sorry
+
+lemma le_TC_trans [trans]: 
+  assumes "X \<le> Y"
+  and "Y \<le> Z"
+shows "X \<le> Z"
+  using assms lt_if_lt_if_mem_strong  lt_iff_mem_trans_closure unfolding le_iff_mem_trans_closure_or_eq  by auto
+
 
 lemma not_lt_self [iff]: "\<not>(X < X)"
   using lt_iff_mem_trans_closure by auto
