HOTG/Arithmetics/Arithmetics.thy
@@ -1,6 +1,8 @@
 theory Arithmetics
   imports
     Set_Add
+    Replacement
+    Less_Than
 begin
 
 paragraph \<open>Summary\<close>
@@ -18,6 +20,11 @@ unbundle hotg_mul_syntax
 
 lemma mul_eq_union_repl_lift_mul: "X * Y = \<Union>{lift (X * y) X | y \<in> Y}"
   by (auto simp:mul_def transrec_eq)
+
+lemma elts_multE:
+  assumes "z \<in> (X * Y)"
+  obtains u v where "u \<in> X" "v \<in> Y" "z = X * v + u"
+ using mul_eq_union_repl_lift_mul[of X Y] assms lift_eq_image_add by auto
 
 lemma mul_zero_eq_zero [simp]: "x * 0 = 0"
   unfolding mul_def by (auto simp: transrec_eq)
@@ -43,9 +50,27 @@ proof -
   finally show ?thesis .
 qed
 
+lemma mul_bin_union_eq_bin_union_mul: "X * (Y \<union> Z) = (X * Y) \<union> (X * Z)"
+proof-
+  have "X * (Y \<union> Z) = \<Union>{lift (X * y) X | y \<in> (Y \<union> Z)}"
+    by (subst mul_eq_union_repl_lift_mul) simp
+  also have "... = \<Union>{lift (X * y) X | y \<in> Y} \<union> \<Union>{lift (X * y) X | y \<in> Z}" by blast
+  also have "... = (X * Y) \<union> (X * Z)" by (simp flip: mul_eq_union_repl_lift_mul)
+  finally show ?thesis .
+qed
+
 lemma mul_insert_eq_mul_bin_union_lift_mul:
   "X * (insert Z Y) = (X * Y) \<union> lift (X * Z) X"
-  sorry
+proof -
+  have mul_set:"X * {Z} = lift (X * Z) X"
+    by (auto simp: mul_eq_union_repl_lift_mul[of _ "{Z}"])
+  have "X * (insert Z Y) = X * (Y \<union> {Z})" by auto
+  also have "... = (X * Y) \<union> (X * {Z})"
+    by (simp only: mul_bin_union_eq_bin_union_mul[of _ _ "{Z}"])
+  also have "... = (X * Y) \<union> lift (X * Z) X"
+    by (auto simp: mul_set)
+  finally show "X * (insert Z Y) = (X * Y) \<union> lift (X * Z) X" .
+qed
 
 lemma mul_add_one_eq_mul_add [simp]:
   "X * (Y + 1) = X * Y + X"
@@ -65,41 +90,36 @@ proof (induction X)
   then show ?case by (auto simp: mul_eq_union_repl_lift_mul[where ?Y = x])
 qed
 
-lemma mul_bin_union_eq_bin_union_mul: "X * (Y \<union> Z) = (X * Y) \<union> (X * Z)"
-proof-
-  have "X * (Y \<union> Z) = \<Union>{lift (X * y) X | y \<in> (Y \<union> Z)}"
-    by (subst mul_eq_union_repl_lift_mul) simp
-  also have "... = \<Union>{lift (X * y) X | y \<in> Y} \<union> \<Union>{lift (X * y) X | y \<in> Z}" by blast
-  also have "... = (X * Y) \<union> (X * Z)" by (simp flip: mul_eq_union_repl_lift_mul)
-  finally show ?thesis .
-qed
+lemma union_repl_distri: 
+  shows "{f x | x \<in> \<Union>X} = \<Union>(repl X (\<lambda>Y. {f x | x \<in> Y})) "
+  sorry
 
-lemma mul_union_eq_union_mul: "X * \<Union>Y = \<Union>(X * Y)"
+lemma mul_union_eq_union_mul: "X * \<Union>Y = \<Union>(repl Y ((*) X))"
 proof-
+  have 1:"(\<lambda>Y. \<Union>{lift (X * y) X | y \<in> Y})  = (\<lambda>Y. (*) X Y)"
+    by (subst mul_eq_union_repl_lift_mul) auto
+  then have 2: "repl Y (\<lambda>Y. \<Union>{lift (X * y) X | y \<in> Y})  = repl Y (\<lambda>Y. (*) X Y)"
+    by (auto simp: arg_cong[of "(\<lambda>Y. \<Union>{lift (X * y) X | y \<in> Y})" "(*) X"])
   have "X * (\<Union>Y) = \<Union>{lift (X * y) X | y \<in> (\<Union>Y)}"
     by (subst mul_eq_union_repl_lift_mul) auto
-  also have "... = \<Union>\<Union>{lift (X * y) X | y \<in> Y}"
-    sorry
-  also have "... = \<Union>(X * Y)"
-    by (subst mul_eq_union_repl_lift_mul) auto
+  also have "... = \<Union>(repl Y (\<lambda>Y. \<Union>{lift (X * y) X | y \<in> Y}))"
+    by (auto simp: union_repl_distri)
+  also have "... = \<Union>(repl Y ((*) X))"
+    by (auto simp: 2 arg_cong[of "(repl Y (\<lambda>Y. \<Union>{lift (X * y) X | y \<in> Y}))" "(repl Y ((*) X))"])
   finally show ?thesis .
 qed
-
-lemma unfolding_mul_union_eq_union_mul:
-  "\<Union>{X * lift(Y * z) Y | z \<in> Z} = X * \<Union>{lift(Y * z) Y | z \<in> Z}"
-  sorry
 
 lemma mul_lift_eq_lift_mul_mul: "X * (lift Y Z) = lift (X * Y) (X * Z)"
 proof(induction Z rule:mem_induction)
   case (mem Z)
+  have sub:"\<Union>{lift (X * (Y + z)) X | z \<in> Z} = \<Union>{lift (X * Y + X * z) X| z \<in> Z }"
+    by (auto simp: mem add_eq_bin_union_lift  mul_bin_union_eq_bin_union_mul)
   have "X * (lift Y Z) = \<Union>{lift (X * z) X | z \<in> (lift Y Z)}"
     by (subst mul_eq_union_repl_lift_mul) auto
   also have "... = \<Union>{lift (X * (Y + z)) X | z \<in> Z}"
-    sorry
-  also have "... = \<Union>{lift (X * Y + X * z) X | z \<in> Z}"
-    sorry
+    by (simp add: lift_eq_image_add)
   also have "... = lift (X * Y) (\<Union>{ lift  (X * z) X  | z \<in> Z})"
-    by (auto simp: lift_union_eq_union_repl_lift lift_lift_eq_lift_add)
+    by (auto simp: sub lift_union_eq_union_repl_lift lift_lift_eq_lift_add)
   also have "... = lift (X * Y) (X * Z)"
     by (subst mul_eq_union_repl_lift_mul) auto
   finally show ?case .
@@ -116,10 +136,80 @@ proof(induction Z rule:mem_induction)
   also have "... = \<Union>{X * lift(Y * z) Y | z \<in> Z}"
     by (auto simp: mem mul_lift_eq_lift_mul_mul)
   also have "... = X * \<Union>{lift(Y * z) Y | z \<in> Z}"
-    by (auto simp: unfolding_mul_union_eq_union_mul)
+    by (auto simp: mul_union_eq_union_mul)
   also have "... = X * (Y * Z)"
     by (subst mul_eq_union_repl_lift_mul) auto
   finally show ?case .
 qed
+
+lemma le_add: "X \<le> X + Y"
+proof-
+  have "X \<in> mem_trans_closure (X + Y) \<or> X = (X + Y)" 
+  proof(cases "Y = 0")
+    case False
+    then show ?thesis sorry
+  qed auto
+  then show ?thesis by (simp add: le_iff_mem_trans_closure_or_eq)
+qed
+
+lemma le_mul_if_not_zero: assumes "Y \<noteq> 0"  
+  shows "X \<le> X * Y"
+proof (cases "X = 0")
+  case False
+  then show ?thesis  
+  proof (induction Y rule:mem_induction)
+    case (mem Y)
+    then show ?case
+    proof (cases "Y = 1")
+      case False
+      obtain P where P: "P \<in> Y"  "P \<noteq> 0" 
+        sorry
+      have ineq_1:"X \<le> X * P" using P mem by auto
+      obtain R where R: "R \<in> X" using \<open>X \<noteq> 0\<close> by auto
+      then have "X * P + R \<in> lift (X * P) X"
+        by (auto simp: lift_eq_image_add)
+      moreover  have "lift (X * P) X \<subseteq> X * Y"
+        using P(1) by (auto simp:mul_eq_union_repl_lift_mul[of _ Y])
+      ultimately have ineq_3:"X * P + R \<le> X * Y"
+        by (auto simp: le_iff_mem_trans_closure_or_eq mem_mem_trans_closure_if_mem)
+      moreover have ineq_2:"X * P \<le> X * P + R"
+        by (auto simp: le_add)
+      then show ?thesis 
+        using ineq_1 ineq_2 ineq_3 le_TC_trans by blast
+    qed (auto simp:le_iff_mem_trans_closure_or_eq)
+  qed
+qed (auto simp:le_iff_mem_trans_closure_or_eq)
+
+lemma sevenn: assumes "R < A" "S < A" "A * X + R \<subseteq> A * Y + S"
+  shows "X \<subseteq> Y"
+  sorry
+
+lemma seven: assumes "R < A" "S < A" "A * X + R = A * Y + S"
+  shows "X = Y" "R = S"
+  sorry
+
+lemma bin_inter_lift_mul_TC_lift_mul_TC_eq_zero:
+  assumes "X \<noteq> Y"
+  shows "lift (A * X) (mem_trans_closure A) \<inter> lift (A * Y) (mem_trans_closure A) = 0"
+proof -
+  have "lift (A * X) (mem_trans_closure A) \<inter> lift (A * Y) (mem_trans_closure A) \<subseteq> 0"
+  proof(rule subsetI)
+    have 1:"lift (A * X) (mem_trans_closure A) = {A * X + r | r \<in> mem_trans_closure A}"
+           "lift (A * Y) (mem_trans_closure A) = {A * Y + r | r \<in> mem_trans_closure A}"
+      by (auto simp: lift_eq_repl_add)
+    fix x assume "x \<in> lift (A * X) (mem_trans_closure A) \<inter> lift (A * Y) (mem_trans_closure A)"
+    then have 2:"x \<in> lift (A * X) (mem_trans_closure A)" "x \<in> lift (A * Y) (mem_trans_closure A)" by auto
+    then obtain r where R:"x = A * X + r" "A * X + r \<in> lift (A * X) (mem_trans_closure A)" "r \<in> mem_trans_closure A"
+      using 1 by auto
+    then obtain rr where RR:"x = A * Y + rr" "A * Y + rr \<in> lift (A * Y) (mem_trans_closure A)" "rr \<in> mem_trans_closure A"
+      using 1 2 by auto
+    with R have "A * X + r = A * Y + rr" "r < A" "rr < A" 
+      by (auto simp:lt_iff_mem_trans_closure  lift_eq_repl_add)
+    then have "X = Y" "r = rr" using seven[of r _ rr X _]  by auto
+    then show "x \<in> 0" by (simp add:assms)
+  qed
+  then show ?thesis by simp
+qed
+
 
 end
